Proved preservation lemma using a decreasing measure.

src/SimulationUtils.v
@@ -1,5 +1,6 @@
 Require Import RelationClasses.
 Require Import PathToSubtree.
+Require Import Arith.
 
 (* The general definition of forward simulation. That means that for all a >= b (with
    a : A and b : B) and a -> c (with c : C), then there exists d : D that completes
@@ -38,6 +39,28 @@ Global Instance transitive_refl_trans_closure A (R : A -> A -> Prop) :
   Transitive (refl_trans_closure R).
 Proof. intros ? ? ?. apply Cl_trans. Qed.
 
+Lemma refl_trans_closure_ind_left A R (P : A -> A -> Prop)
+  (Prefl : forall a : A, P a a)
+  (Pstep : forall a b c, R a b -> refl_trans_closure R b c -> P b c -> P a c) :
+  forall a b, refl_trans_closure R a b -> P a b.
+Proof.
+  intros a b rel_a_b.
+  assert (forall c, refl_trans_closure R b c -> P b c -> P a c).
+  { induction rel_a_b; debug eauto using Cl_trans. }
+  auto using Cl_refl.
+Qed.
+
+Lemma refl_trans_closure_ind_right A R (P : A -> A -> Prop)
+  (Prefl : forall a : A, P a a)
+  (Pstep : forall a b c, refl_trans_closure R a b -> P a b -> R b c -> P a c) :
+  forall a b, refl_trans_closure R a b -> P a b.
+Proof.
+  intros b c rel_b_c.
+  assert (forall a, refl_trans_closure R a b -> P a b -> P a c).
+  { induction rel_b_c; debug eauto using Cl_trans. }
+  auto using Cl_refl.
+Qed.
+
 (* Generally, to prove preservation when the relation is a reflexive transitive closure, it
  * suffices to prove it for the base cases. *)
 Lemma preservation_by_base_case {A B : Type}
@@ -53,6 +76,62 @@ Proof.
     destruct (IH1 _ Red_a0_b0) as (b1 & ? & Red_a1_b1).
     destruct (IH0 _ Red_a1_b1) as (b2 & ? & Red_a2_b2).
     exists b2. split; [ | assumption]. transitivity b1; assumption.
+Qed.
+
+(* Reorganizations and le are defined as reflexive-transitive closure of relations (that we are
+ * going to denote < and reorg). When we want to prove the preservation, ie:
+
+    Sl <*  Sr
+
+    |      |
+    *      *
+    v      v
+
+   Sl' <* Sr'
+
+ * We want to derive it by only considering the cases of < and reorg, and ignoring the reflexive and 
+ * transitive cases:
+
+    Sl <  Sr
+
+    |     |
+    *     |
+    v     v
+
+   Sl' <* Sr'
+
+ * However, this proof scheme is wrong in general. Our strategy is to exhibit a measure |.| from
+ * states to a well-founded order, that is decreasing by applications of < and reorg.
+ *)
+(* Note: for the moment, we just use natural measures. *)
+Lemma preservation_reorg A (le reorg : A -> A -> Prop) (measure : A -> nat)
+  (le_decreasing : forall a b, le a b -> measure a < measure b)
+  (reorg_decreasing : forall a b, reorg a b -> measure b < measure a)
+  (H : forward_simulation le (refl_trans_closure le) reorg (refl_trans_closure reorg)) :
+  forward_simulation (refl_trans_closure le) (refl_trans_closure le) (refl_trans_closure reorg) (refl_trans_closure reorg).
+Proof.
+  assert (forall S S', refl_trans_closure reorg S S' -> measure S' <= measure S).
+  { intros ? ? Hreorg. induction Hreorg; eauto using Nat.lt_le_incl, Nat.le_trans. }
+  intros Sr.
+  remember (measure Sr) as n eqn:EQN. revert Sr EQN.
+  induction n as [? IH] using lt_wf_ind.
+  intros Sr -> Sr' reorg_Sr_Sr'.
+  destruct reorg_Sr_Sr' as [ | Sr Sr' Sr'' reorg_Sr_Sr' ? _] using refl_trans_closure_ind_left.
+  { intros. eexists. split; [eassumption | reflexivity]. }
+  intros Sl le_Sl_Sr.
+  destruct le_Sl_Sr as [ | Sl Sm Sr ? _ le_Sm_Sr] using refl_trans_closure_ind_right.
+  { eexists. split; [reflexivity | ]. transitivity Sr'; [constructor | ]; assumption. }
+  specialize (H _ _ reorg_Sr_Sr' _ le_Sm_Sr). destruct H as (Sm' & le_Sm'_Sr' & reorg_Sm_Sm').
+  assert (exists Sl', refl_trans_closure le Sl' Sm' /\ refl_trans_closure reorg Sl Sl')
+    as (Sl' & ? & ?)
+    by eauto.
+  assert (exists Sm'', refl_trans_closure le Sm'' Sr'' /\ refl_trans_closure reorg Sm' Sm'')
+    as (Sm'' & ? & ?)
+    by eauto.
+  assert (exists Sl'', refl_trans_closure le Sl'' Sm'' /\ refl_trans_closure reorg Sl' Sl'')
+    as (? & ? & ?).
+  { eapply IH; [ | reflexivity | eassumption..]. eauto using Nat.le_lt_trans. }
+  eexists. split; [transitivity Sm'' | transitivity Sl']; eassumption.
 Qed.
 
 (* Generally, to complete the square diagram, we will prove that:
@@ -87,7 +166,9 @@ Class LeBase (B V : Type) := {
   le_base : state B V -> state B V -> Prop;
   well_formed : state B V ->  Prop;
   anon : B;
-  le_base_preserves_well_formedness Sl Sr : well_formed Sr -> le_base Sl Sr -> well_formed Sl
+  le_base_preserves_well_formedness Sl Sr : well_formed Sr -> le_base Sl Sr -> well_formed Sl;
+  measure : state B V -> nat;
+  le_base_decreases_measure Sl Sr : le_base Sl Sr -> measure Sl < measure Sr
 }.
 
 (* A restriction of a relation to the set of well-formed states *)
@@ -141,6 +222,54 @@ Proof.
   - specialize (IH1 WF_Sr). destruct IH1 as (WF_Sm & ?).
     specialize (IH0 WF_Sm). destruct IH0.
     eexists. etransitivity; eassumption.
+Qed.
+
+Lemma forward_simulation_right_covariant A (le red0 red1 : A -> A -> Prop)
+  (sub_red1_red0 : forall a b, red0 a b -> red1 a b) :
+  forward_simulation le le red0 red0 -> forward_simulation le le red0 red1.
+Proof.
+  intros H a b ? c ?. edestruct H as (d & ? & ?). eassumption. eassumption.
+  exists d. split. assumption. eauto.
+Qed.
+
+Lemma forward_simulation_left_contravariant A (le red0 red1 : A -> A -> Prop)
+  (sub_red1_red0 : forall a b, red1 a b -> red0 a b) :
+  forward_simulation le le red0 red1 -> forward_simulation le le red1 red1.
+Proof. unfold forward_simulation. eauto. Qed.
+
+Corollary preservation_invariant A (le red0 red1 : A -> A -> Prop)
+  (equiv_red0_red1 : forall a b, red0 a b <-> red1 a b) :
+  forward_simulation le le red0 red0 -> forward_simulation le le red1 red1.
+Proof.
+  intro.
+  apply forward_simulation_left_contravariant with (red0 := red0). { firstorder. }
+  apply forward_simulation_right_covariant with (red0 := red0). { firstorder. }
+  assumption.
+Qed.
+
+(* When proving preservation on well-formed states, we can use an additional hypothesis on
+   the base case: that the state Sr (such that Sl <= Sr) is well-formed. *)
+Lemma preservation_by_base_case_reorg B V `(LB : LeBase B V)
+  (reorg : state B V -> state B V -> Prop)
+  (reorg_decreases_measure : forall S S', reorg S S' -> measure S' < measure S) :
+  (forall Sr Sr', reorg Sr Sr' -> @well_formed _ _ LB Sr -> forall Sl, @le_base _ _ LB Sl Sr
+   -> exists Sl', @le _ _ (@LeState _ _ LB) Sl' Sr' /\ (refl_trans_closure reorg) Sl Sl')
+  -> @preservation _ _ (@LeStateWF _ _ LB) (@LeStateWF _ _ LB) (restrict (refl_trans_closure reorg)).
+Proof.
+  intros simulation.
+  (* Je suppose que sous la condition que reorg préserve la bonne formation, on peut
+     commuter restrict et refl_trans_closure. *)
+  apply preservation_invariant with (red0 := refl_trans_closure (restrict reorg)).
+  { admit. }
+  apply preservation_reorg with (measure := fun S => measure (proj1_sig S)).
+  { intros (Sl & ?) (Sr & ?). apply le_base_decreases_measure. }
+  { intros (Sl & ?) (Sr & ?) Hreorg. destruct Hreorg. apply reorg_decreases_measure. assumption. }
+  intros Sr Sr' red_Sr_Sr' (Sl & WF_Sl) Hle.
+  destruct red_Sr_Sr' as [(Sr & WF_Sr) Sr' red_Sr_Sr']. cbn in red_Sr_Sr'.
+  edestruct (simulation _ _ red_Sr_Sr') as (Sl' & le_Sl'_Sr' & red_Sl_Sl'); [eassumption.. | ].
+  apply preservation_state_implies_preservation_restriction in le_Sl'_Sr'.
+  destruct le_Sl'_Sr' as (WF_Sl' & le_Sl'_Sr').
+  exists (exist _ Sl' WF_Sl'). split. assumption. 
 Qed.
 
 (* When proving preservation on well-formed states, we can use an additional hypothesis on
